proofs/fstar/extraction/Libcrux.Kem.Kyber.Kyber1024.fst
@@ -3,21 +3,36 @@ module Libcrux.Kem.Kyber.Kyber1024
 open Core
 open FStar.Mul
 
-let decapsulate_1024_
+let decapsulate
       (secret_key: Libcrux.Kem.Kyber.Types.t_MlKemPrivateKey (sz 3168))
       (ciphertext: Libcrux.Kem.Kyber.Types.t_MlKemCiphertext (sz 1568))
      =
   Libcrux.Kem.Kyber.decapsulate (sz 4) (sz 3168) (sz 1536) (sz 1568) (sz 1568) (sz 1536) (sz 1408)
     (sz 160) (sz 11) (sz 5) (sz 352) (sz 2) (sz 128) (sz 2) (sz 128) (sz 1600) secret_key ciphertext
 
-let encapsulate_1024_
+let encapsulate
       (public_key: Libcrux.Kem.Kyber.Types.t_MlKemPublicKey (sz 1568))
       (randomness: t_Array u8 (sz 32))
      =
   Libcrux.Kem.Kyber.encapsulate (sz 4) (sz 1568) (sz 1568) (sz 1536) (sz 1408) (sz 160) (sz 11)
     (sz 5) (sz 352) (sz 2) (sz 128) (sz 2) (sz 128) public_key randomness
 
-let generate_key_pair_1024_ (randomness: t_Array u8 (sz 64)) =
+let validate_public_key (public_key: Libcrux.Kem.Kyber.Types.t_MlKemPublicKey (sz 1568)) =
+  if
+    Libcrux.Kem.Kyber.validate_public_key (sz 4)
+      (sz 1536)
+      (sz 1568)
+      public_key.Libcrux.Kem.Kyber.Types.f_value
+  then
+    Core.Option.Option_Some public_key
+    <:
+    Core.Option.t_Option (Libcrux.Kem.Kyber.Types.t_MlKemPublicKey (sz 1568))
+  else
+    Core.Option.Option_None
+    <:
+    Core.Option.t_Option (Libcrux.Kem.Kyber.Types.t_MlKemPublicKey (sz 1568))
+
+let generate_key_pair (randomness: t_Array u8 (sz 64)) =
   Libcrux.Kem.Kyber.generate_keypair (sz 4)
     (sz 1536)
     (sz 3168)
